progress with ground atom ID logic

Grounded_PDDL.thy
@@ -4,7 +4,8 @@ imports "AI_Planning_Languages_Semantics.PDDL_STRIPS_Semantics"
     Utils String_Shenanigans
 begin
 
-type_synonym facty = "object atom formula"
+type_synonym facty = "object atom formula" (* maybe fact_atom? *)
+
 
 (* TODO split into wf_dom_grounder, dom_grounder, prob_grounder? *)
 
@@ -38,11 +39,11 @@ definition "fact_prefix_pad \<equiv> length (show (length facts))" (* length fac
 definition "op_ids \<equiv> nat_range (length ops)"
 definition "op_prefix_pad \<equiv> length (show (length ops))" (* length ops - 1 is enough *)
 
-fun grounded_pred :: "facty \<Rightarrow> nat \<Rightarrow> predicate" where
-  "grounded_pred (Atom a) i = Pred (padl fact_prefix_pad (show i) @ (CHR ''/'' # fact_str a))" |
-  "grounded_pred _ _ = undefined"
+fun ground_pred :: "facty \<Rightarrow> nat \<Rightarrow> predicate" where
+  "ground_pred (Atom a) i = Pred (padl fact_prefix_pad (show i) @ (CHR ''/'' # fact_str a))" |
+  "ground_pred _ _ = undefined"
 
-abbreviation "gr_pred_ids \<equiv> map2 grounded_pred facts fact_ids"
+abbreviation "gr_pred_ids \<equiv> map2 ground_pred facts fact_ids"
 definition "fact_map \<equiv> map_of (zip (map un_Atom facts) gr_pred_ids)"
 
 fun map_fact :: "object atom \<Rightarrow> 'a atom" where
@@ -62,8 +63,8 @@ fun ground_ac_name :: "plan_action \<Rightarrow> nat \<Rightarrow> string" where
   "ground_ac_name (PAction n args) i =
     pad op_prefix_pad (show i) @ (CHR ''/'' # n) @ ((CHR ''-'' # arg_str args))"
 
-fun grounded_ac :: "plan_action \<Rightarrow> nat \<Rightarrow> ast_action_schema" where
-  "grounded_ac \<pi> i =
+definition ground_ac :: "plan_action \<Rightarrow> nat \<Rightarrow> ast_action_schema" where
+  "ground_ac \<pi> i =
     (let ga = resolve_instantiate \<pi> in
     Action_Schema (ground_ac_name \<pi> i) [] (ga_pre ga) (ga_eff ga))"
 
@@ -72,7 +73,7 @@ definition ground_dom :: "ast_domain" where
     []
     (map (\<lambda>p. PredDecl p []) gr_pred_ids)
     []
-    (map2 grounded_ac ops op_ids)"
+    (map2 ground_ac ops op_ids)"
 
 definition ground_prob :: "ast_problem" where
   "ground_prob \<equiv> Problem
@@ -97,16 +98,182 @@ locale wf_grounder = grounder +
     wf_problem and
     facts_dist: "distinct facts" and
     all_facts: "set facts \<supseteq> {a. achievable a}" and
+    facts_wf: "list_all1 (wf_fmla_atom objT) facts" and (* If "set facts = {a. achievable a}", this follows. *)
     ops_dist: "distinct ops" and
-    ops_correct: "set ops \<supseteq> {\<pi>. applicable \<pi>}"
-begin end
+    ops_correct: "set ops \<supseteq> {\<pi>. applicable \<pi>}" and
+    ops_wf: "list_all1 wf_plan_action ops" (* If "set ops = {\<pi>. applicable \<pi>}", this follows. *)
+
+abbreviation (in grounder) "D\<^sub>G \<equiv> ground_dom"
+abbreviation (in grounder) "P\<^sub>G \<equiv> ground_prob"
 
 sublocale wf_grounder \<subseteq> wf_ast_problem P
   apply (unfold_locales)
   using wf_grounder_axioms wf_grounder_def by blast
 
+sublocale grounder \<subseteq> dg: ast_domain D\<^sub>G .
+sublocale grounder \<subseteq> pg: ast_problem P\<^sub>G .
 
-subsection \<open> locale setup \<close>
+subsection \<open> Alternative definitions \<close>
+
+context grounder begin
+
+find_theorems "(?x = predAtm ?a ?b \<Longrightarrow> ?P)"
+
+lemma ground_pred_cond:
+  "is_predAtom a \<Longrightarrow>
+  (\<exists>s. ground_pred a i = Pred (padl fact_prefix_pad (show i) @ s))"
+  by (cases a rule: is_predAtom.cases) simp_all
+
+lemma ga_pre_alt: "ga_pre ga = map_formula map_fact (precondition ga)"
+  by (cases ga; simp)
+
+lemma ga_eff_alt: "ga_eff ga =
+  Effect (map (map_formula map_fact) (adds (effect ga))) (map (map_formula map_fact) (dels (effect ga)))"
+  by (cases ga rule: ga_eff.cases) simp
+
+lemma ga_eff_sel [simp]:
+  "adds (ga_eff ga) = map (map_formula map_fact) (adds (effect ga))"
+  "dels (ga_eff ga) = map (map_formula map_fact) (dels (effect ga))"
+  unfolding ga_eff_alt by simp_all
+
+lemma ground_ac_sel [simp]:
+  "ac_name (ground_ac \<pi> i) = ground_ac_name \<pi> i"
+  "ac_params (ground_ac \<pi> i) = []"
+  "ac_pre (ground_ac \<pi> i) = ga_pre (resolve_instantiate \<pi>)"
+  "ac_eff (ground_ac \<pi> i) = ga_eff (resolve_instantiate \<pi>)"
+  unfolding ground_ac_def Let_def by simp_all
+
+lemma ground_dom_sel [simp]:
+  "types D\<^sub>G = []"
+  "predicates D\<^sub>G = map (\<lambda>p. PredDecl p []) gr_pred_ids"
+  "consts D\<^sub>G = []"
+  "actions D\<^sub>G = map2 ground_ac ops op_ids"
+  unfolding ground_dom_def by simp_all
+
+lemma ground_prob_sel [simp]:
+  "domain P\<^sub>G \<equiv> D\<^sub>G"
+  "objects P\<^sub>G = []"
+  "init P\<^sub>G = map (map_formula map_fact) (init P)"
+  "goal P\<^sub>G = map_formula map_fact (goal P)"
+  unfolding ground_prob_def by simp_all
+
+lemma restore_ground_pa_alt: "restore_ground_pa \<pi> = the (pa_map (name \<pi>))"
+  by (cases \<pi>) simp
+
+end
+
+subsection \<open> Output format \<close>
+text \<open> The output is, in fact, grounded \<close>
+
+context grounder begin
+
+lemma acs_grounded: "list_all1 grounded_ac (actions D\<^sub>G)"
+proof
+  fix x assume a: "x \<in> set (actions D\<^sub>G)"
+  then obtain op i where "x = ground_ac op i" by auto
+  hence "ac_params x = []" by simp
+  thus "grounded_ac x" by (cases x) simp
+qed
+
+theorem ground_dom_grounded: "dg.grounded_dom"
+  unfolding dg.grounded_dom_def apply (intro conjI)
+     apply simp
+  unfolding grounded_pred.simps apply (intro ballI)
+  subgoal for x apply (cases x) by auto
+   apply simp
+  using acs_grounded by blast
+
+theorem ground_prob_grounded: "pg.grounded_prob"
+  using pg.grounded_prob_def ground_dom_grounded by simp
+
+end
+
+subsection \<open> Well-formedness \<close>
+
+context grounder begin
+end
+
+(* TODO \<rightarrow> Utils *)
+lemma map2_obtain:
+  assumes "z \<in> set (map2 f xs ys)"
+  obtains x y where "z = f x y" "x \<in> set xs" "y \<in> set ys"
+  using assms by (induction xs ys rule: list_induct2') auto
+
+(* TODO \<rightarrow> Utils *)
+lemma map2_dist_2:
+  assumes "distinct ys" "\<And>x1 x2 y1 y2. y1 \<in> set ys \<Longrightarrow> y2 \<in> set ys \<Longrightarrow> y1 \<noteq> y2 \<Longrightarrow> f x1 y1 \<noteq> f x2 y2"
+  shows "distinct (map2 f xs ys)"
+  using assms proof (induction xs ys rule: list_induct2')
+  case (4 x xs y ys)
+  hence "distinct (map2 f xs ys)" by simp
+
+  thus ?case apply (induction xs ys rule: list_induct2') oops
+
+context wf_grounder begin
+
+lemma gr_preds_dis: "distinct (map pred (predicates D\<^sub>G))"
+proof -
+
+  have "gr_pred_ids ! i \<noteq> gr_pred_ids ! j" if "i \<noteq> j" "i < length (gr_pred_ids)" "j < length (gr_pred_ids)" for i j
+  proof -
+    have len: "length gr_pred_ids = length facts"
+      unfolding fact_ids_def using nat_range_length by simp
+    hence nth: "gr_pred_ids ! x = ground_pred (facts ! x) x" if "x < length facts" for x
+      unfolding fact_ids_def using that nat_range_nth by simp
+
+    have "is_predAtom (facts ! x)" if "x < length facts" for x
+      using facts_wf wf_fmla_atom_alt that by fastforce
+    with nth have app: "\<exists>s. gr_pred_ids ! x = Pred (padl fact_prefix_pad (show x) @ s)" if "x < length facts" for x
+      using that ground_pred_cond by simp
+    have "length (padl fact_prefix_pad (show x)) = fact_prefix_pad" if "x < length facts" for x
+      using that fact_prefix_pad_def padl_length nat_show_len_mono
+      using order_less_imp_le by metis
+    hence "padl fact_prefix_pad (show i) @ s \<noteq> padl fact_prefix_pad (show j) @ t" for s t
+      using that pad_show_neq by simp
+    thus ?thesis using that app len by (metis predicate.inject)
+  qed
+  hence "distinct gr_pred_ids" using distinct_conv_nth by blast
+  moreover have "map pred (predicates D\<^sub>G) = gr_pred_ids" by simp
+  ultimately show ?thesis by metis
+qed
+
+lemma gr_preds_wf: "list_all1 pg.wf_predicate_decl (predicates D\<^sub>G)"
+  sorry
+lemma gr_acs_dis: "distinct (map ac_name (actions D\<^sub>G))"
+  sorry
+lemma gr_acs_wf: "list_all1 pg.wf_action_schema (actions D\<^sub>G)"
+  sorry
+
+theorem ground_dom_wf: "dg.wf_domain"
+  unfolding dg.wf_domain_def apply (intro conjI)
+  using dg.wf_types_def apply simp
+  using gr_preds_dis apply simp
+  using gr_preds_wf apply simp
+  apply simp (* consts wf *)
+  apply simp (* consts' types *)
+  using gr_acs_dis gr_acs_wf by simp_all
+
+theorem ground_prob_wf: "pg.wf_problem"
+  unfolding pg.wf_problem_def apply (intro conjI)
+  using ground_dom_wf apply simp
+      apply simp (* consts + objects distinct *)
+     apply simp (* objects' types *)
+  oops
+
+
+end
+
+sublocale wf_grounder \<subseteq> dg: wf_ast_domain D\<^sub>G
+  using ground_dom_wf
+  by (simp add: wf_ast_domain_def)
+
+sublocale wf_grounder \<subseteq> pg: wf_ast_problem P\<^sub>G
+  oops
+
+
+subsection \<open> Semantics \<close>
+
+text \<open> ground locale setup \<close>
 
 locale grounded_domain = wf_ast_domain +
   assumes grounded_dom: grounded_dom
@@ -144,11 +311,11 @@ lemmas pddl_ground_code =
   grounder.fact_prefix_pad_def
   grounder.op_ids_def
   grounder.op_prefix_pad_def
-  grounder.grounded_pred.simps
+  grounder.ground_pred.simps
   grounder.map_fact.simps
   grounder.ga_pre.simps
   grounder.ga_eff.simps
-  grounder.grounded_ac.simps
+  grounder.ground_ac_def
   grounder.ground_dom_def
   grounder.ground_prob_def
   grounder.ground_ac_name.simps
